Expansion.thy
@@ -1,0 +1,274 @@
+theory Expansion
+  imports Context_Free_Grammar.Context_Free_Grammar "Regular-Sets.Regular_Set"
+begin
+
+lemma insert_conc: "insert w W @@ V = {w @ v | v. v \<in> V} \<union> W @@ V"
+  by auto
+
+text \<open>Language is extended over mixed words.\<close>
+
+definition Lang_of where
+"Lang_of P \<alpha> = {w. P \<turnstile> \<alpha> \<Rightarrow>* map Tm w}"
+
+lemma Lang_of_Nil[simp]: "Lang_of P [] = {[]}"
+  by (auto simp: Lang_of_def)
+
+lemma Lang_of_iff_derives: "w \<in> Lang_of P \<alpha> \<longleftrightarrow> P \<turnstile> \<alpha> \<Rightarrow>* map Tm w"
+  by (auto simp: Lang_of_def)
+
+lemma Lang_eq_iff_Lang_of_eq: "Lang P = Lang P' \<longleftrightarrow> Lang_of P = Lang_of P'"
+  by (unfold Lang_eq_iff_derives, auto simp: fun_eq_iff Lang_of_def)
+
+lemma Lang_of_Tm: "Lang_of P (Tm a # \<alpha>) = {[a]} @@ Lang_of P \<alpha>"
+  by (auto simp: Lang_of_def derives_Tm_Cons conc_def)
+
+lemma Lang_of_map_Tm: "Lang_of P (map Tm w) = {w}"
+  by (induction w, simp_all add: Lang_of_Tm insert_conc)
+
+lemma Lang_of_Nt: "Lang_of P (Nt A # \<alpha>) = Lang P A @@ Lang_of P \<alpha>"
+  by (force simp add: Lang_of_def Lang_def derives_Cons_decomp map_eq_append_conv conc_def)
+
+lemma Lang_of_Cons: "Lang_of P (x # \<alpha>) = (case x of Tm a \<Rightarrow> {[a]} | Nt A \<Rightarrow> Lang P A) @@ Lang_of P \<alpha>"
+  by (simp add: Lang_of_Tm Lang_of_Nt split: sym.splits)
+
+lemma Lang_of_append: "Lang_of P (\<alpha> @ \<beta>) = Lang_of P \<alpha> @@ Lang_of P \<beta>"
+  by (induction \<alpha> arbitrary: \<beta>, simp_all add: Lang_of_Cons conc_assoc split: sym.splits)
+
+abbreviation Lang_of_set where
+"Lang_of_set P X \<equiv> \<Union>(Lang_of P ` X)"
+
+lemma Lang_of_set_conc: "Lang_of_set P (X @@ Y) = Lang_of_set P X @@ Lang_of_set P Y"
+  by (force simp: Lang_of_append elim!: concE)
+
+lemma Lang_of_set_Rhss: "Lang_of_set P (Rhss P A) = Lang P A"
+  by (auto simp: Lang_def Lang_of_def Rhss_def converse_rtranclp_into_rtranclp derive_singleton
+      dest: derives_start1)
+
+lemma Lang_of_prod_subset: "(A,\<alpha>) \<in> P \<Longrightarrow> Lang_of P \<alpha> \<subseteq> Lang P A"
+  apply (fold Lang_of_set_Rhss) by (auto simp: Rhss_def)
+
+
+lemma Lang_of_set_pow: "Lang_of_set P (X ^^ n) = Lang_of_set P X ^^ n"
+  by (induction n, simp_all add: Lang_of_set_conc)
+
+lemma Lang_of_set_star: "Lang_of_set P (star X) = star (Lang_of_set P X)"
+  by (auto simp: star_def Lang_of_set_pow)
+
+section \<open>General Expansion\<close>
+
+text \<open>We consider the set of admissible expansions of grammars.
+For a symbol,
+one option is not to expand it,
+and another option for (unlocked) nonterminals is to expand to the all rhss.\<close>
+
+definition Expand_sym_ops :: "('n,'t) Prods \<Rightarrow> 'n set \<Rightarrow> ('n,'t) sym \<Rightarrow> ('n,'t) syms set set" where
+"Expand_sym_ops P L x =
+  insert {[x]} (case x of Nt A \<Rightarrow> if A \<in> L then {} else {Rhss P A} | _ \<Rightarrow> {})"
+
+lemma Expand_sym_ops_simps:
+  "Expand_sym_ops P L (Tm a) = {{[Tm a]}}"
+  "Expand_sym_ops P L (Nt A) = insert {[Nt A]} (if A \<in> L then {} else {Rhss P A})"
+  by (auto simp: Expand_sym_ops_def)
+
+lemma Expand_sym_ops_self: "{[x]} \<in> Expand_sym_ops P L x"
+  by (simp add: Expand_sym_ops_def)
+
+text \<open>Mixed words allow all possible combinations of the options of the symbols.\<close>
+
+fun Expand_syms_ops where
+  "Expand_syms_ops P L [] = {{[]}}"
+| "Expand_syms_ops P L (x#xs) =
+   {\<alpha>s @@ \<beta>s | \<alpha>s \<beta>s. \<alpha>s \<in> Expand_sym_ops P L x \<and> \<beta>s \<in> Expand_syms_ops P L xs}"
+
+lemma Expand_sym_ops_Lang_of_Cons:
+  assumes X: "X \<in> Expand_sym_ops P L x"
+    and L: "Lhss Q \<subseteq> L"
+  shows "Lang_of (P \<union> Q) (x#xs) = Lang_of_set (P \<union> Q) X @@ Lang_of (P \<union> Q) xs"
+proof-
+  { fix A assume "A \<notin> L"
+    with L have "A \<notin> Lhss Q" by auto
+    then have "Rhss (P \<union> Q) A = Rhss P A" by (auto simp: Rhss_Un notin_Lhss_iff_Rhss)
+    with Lang_of_set_Rhss[of "P \<union> Q" A]
+    have "Lang_of_set (P \<union> Q) (Rhss P A) = Lang (P \<union> Q) A" by auto
+  } note * = this
+  show ?thesis
+  proof (cases "X = {[x]}")
+    case True
+    with assms show ?thesis by (simp add: Expand_sym_ops_simps Lang_of_Cons)
+  next
+    case False
+    with assms show ?thesis
+      by (cases x, simp_all add: Expand_sym_ops_simps Lang_of_Nt * split: if_splits)
+  qed
+qed
+
+lemma Expand_syms_ops_Lang_of:
+  assumes X: "X \<in> Expand_syms_ops P L \<alpha>"
+    and L: "Lhss Q \<subseteq> L"
+  shows "Lang_of (P \<union> Q) \<alpha> = Lang_of_set (P \<union> Q) X"
+proof (insert X, induction \<alpha> arbitrary: X)
+  case Nil
+  then show ?case by simp
+next
+  case (Cons x \<alpha>)
+  from Cons.prems obtain Y Z
+    where X: "X = Y @@ Z"
+      and Y: "Y \<in> Expand_sym_ops P L x"
+      and Z: "Z \<in> Expand_syms_ops P L \<alpha>"
+    by auto
+  show ?case by (simp add: X Cons.IH[OF Z] Expand_sym_ops_Lang_of_Cons[OF Y L] Lang_of_set_conc)
+qed
+
+definition Expand where
+"Expand f Q = (\<Union>(A,\<alpha>) \<in> Q. Pair A ` f \<alpha>)"
+
+lemma Lhss_Expand: "Lhss (Expand f Q) \<subseteq> Lhss Q"
+  by (auto simp: Lhss_def Expand_def split: prod.splits)
+
+lemma Rhss_Expand: "Rhss (Expand f Q) A = \<Union>(f ` Rhss Q A)"
+  by (auto simp: Rhss_def Expand_def)
+
+text \<open>When each production is expanded in an admissible way,
+then the language is preserved.\<close>
+
+lemma Lang_Expand:
+  assumes f: "\<forall>(A,\<alpha>) \<in> Q. f \<alpha> \<in> Expand_syms_ops P L \<alpha>" and L: "Lhss Q \<subseteq> L"
+  shows "Lang (P \<union> Expand f Q) = Lang (P \<union> Q)"
+proof (intro ext Lang_eqI_derives iffI)
+  have "P \<union> Expand f Q \<turnstile> xs \<Rightarrow>(n) map Tm w \<Longrightarrow> w \<in> Lang_of (P \<union> Q) xs" for xs w n
+  proof (induction n arbitrary: xs w rule: less_induct)
+    case (less n)
+    show ?case
+    proof (cases "\<exists>A. Nt A \<in> set xs")
+      case False
+      with less.prems have "xs = map Tm w"
+        by (metis (no_types, lifting) deriven_from_TmsD destTm.cases ex_map_conv)
+      then show ?thesis by (auto simp: Lang_of_map_Tm)
+    next
+      case True
+      then obtain ys zs A where xs: "xs = ys @ Nt A # zs" by (metis split_list) 
+      from less.prems[unfolded this deriven_Nt_map_Tm]
+      obtain \<delta> m l k v u t where A\<delta>: "(A,\<delta>) \<in> P \<union> Expand f Q"
+        and Lys: "P \<union> Expand f Q \<turnstile> ys \<Rightarrow>(m) map Tm v"
+        and L\<delta>: "P \<union> Expand f Q \<turnstile> \<delta> \<Rightarrow>(l) map Tm u"
+        and Lzs: "P \<union> Expand f Q \<turnstile> zs \<Rightarrow>(k) map Tm t"
+        and n: "n = Suc (m + l + k)"
+        and w: "w = v @ u @ t" by force
+      from n have mn: "m < n" and ln: "l < n" and kn: "k < n" by auto
+      with less.IH L\<delta> Lys Lzs
+      have u: "u \<in> Lang_of (P \<union> Q) \<delta>"
+        and v: "v \<in> Lang_of (P \<union> Q) ys"
+        and t: "t \<in> Lang_of (P \<union> Q) zs" by auto
+      show ?thesis
+      proof (cases "(A,\<delta>) \<in> P")
+        case True
+        have "Lang_of (P \<union> Q) \<delta> \<subseteq> Lang (P \<union> Q) A"
+          apply (rule Lang_of_prod_subset)
+          using True by simp
+        with u v t
+        show ?thesis by (auto simp: xs w Lang_of_append Lang_of_Nt)
+      next
+        case False
+        with A\<delta> obtain \<alpha> where AQ: "(A,\<alpha>) \<in> Q" and \<delta>: "\<delta> \<in> f \<alpha>" by (auto simp: Expand_def)
+        from L\<delta>[unfolded \<delta>] less.IH[of l] n
+        have "u \<in> Lang_of (P \<union> Q) \<delta>" by auto
+        with \<delta> have "u \<in> Lang_of_set (P \<union> Q) (f \<alpha>)"
+          by (auto simp: Lang_of_def)
+        also have "\<dots> = Lang_of (P \<union> Q) \<alpha>"
+          apply (subst Expand_syms_ops_Lang_of)
+          using f AQ L by auto
+        also have "\<dots> \<subseteq> Lang (P \<union> Q) A"
+          apply (rule Lang_of_prod_subset)
+          using AQ by auto
+        finally have u: "u \<in> Lang (P \<union> Q) A" by auto
+        with v t
+        show ?thesis by (simp add: xs w Lang_of_append Lang_of_Nt)
+      qed
+    qed
+  qed
+  then show "P \<union> Expand f Q \<turnstile> xs \<Rightarrow>* map Tm w \<Longrightarrow> P \<union> Q \<turnstile> xs \<Rightarrow>* map Tm w" for xs w
+    by (auto simp: rtranclp_power Lang_of_iff_derives)
+next
+  have "P \<union> Q \<turnstile> xs \<Rightarrow>(n) map Tm w \<Longrightarrow> w \<in> Lang_of (P \<union> Expand f Q) xs" for xs w n
+  proof (induction n arbitrary: xs w rule: less_induct)
+    case (less n)
+    show ?case
+    proof (cases "\<exists>A. Nt A \<in> set xs")
+      case False
+      with less.prems have "xs = map Tm w"
+        by (metis (no_types, lifting) deriven_from_TmsD destTm.cases ex_map_conv)
+      then show ?thesis by (auto simp: Lang_of_map_Tm)
+    next
+      case True
+      then obtain ys zs A where xs: "xs = ys @ Nt A # zs" by (metis split_list) 
+      from less.prems[unfolded this deriven_Nt_map_Tm]
+      obtain \<alpha> m l k v u t where A\<alpha>: "(A,\<alpha>) \<in> P \<union> Q"
+        and Rys: "P \<union> Q \<turnstile> ys \<Rightarrow>(m) map Tm v"
+        and R\<alpha>: "P \<union> Q \<turnstile> \<alpha> \<Rightarrow>(l) map Tm u"
+        and Rzs: "P \<union> Q \<turnstile> zs \<Rightarrow>(k) map Tm t"
+        and n: "n = Suc (m + l + k)"
+        and w: "w = v @ u @ t" by force
+      from n have mn: "m < n" and ln: "l < n" and kn: "k < n" by auto
+      with R\<alpha> Rys Rzs
+      have u: "u \<in> Lang_of (P \<union> Expand f Q) \<alpha>"
+        and v: "v \<in> Lang_of (P \<union> Expand f Q) ys"
+        and t: "t \<in> Lang_of (P \<union> Expand f Q) zs" by (auto simp: less.IH)
+      show ?thesis
+      proof (cases "(A,\<alpha>) \<in> P")
+        case True
+        then have "(A,\<alpha>) \<in> P \<union> Expand f Q" by simp
+        from Lang_of_prod_subset[OF this] u
+        have "u \<in> Lang (P \<union> Expand f Q) A" by auto
+        with v w t
+        show ?thesis by (auto simp: xs w Lang_of_append Lang_of_Nt)
+      next
+        case False
+        with A\<alpha> have A\<alpha>Q: "(A,\<alpha>) \<in> Q" by simp
+        with f have f\<alpha>: "f \<alpha> \<in> Expand_syms_ops P L \<alpha>" by auto
+        from L Lhss_Expand[of f Q]
+        have Lhss: "Lhss (Expand f Q) \<subseteq> L" by auto
+        from L A\<alpha>Q have Rhss: "f \<alpha> \<subseteq> Rhss (Expand f Q) A"
+          by (auto simp: Rhss_def Expand_def)
+        from u Expand_syms_ops_Lang_of[OF f\<alpha> Lhss]
+        have "u \<in> Lang_of_set (P \<union> Expand f Q) (f \<alpha>)" by auto
+        also have "\<dots> \<subseteq> Lang (P \<union> Expand f Q) A" using Rhss
+          by (auto simp flip: Lang_of_set_Rhss simp: Rhss_Un)
+        finally have "u \<in> \<dots>".
+        with v t show ?thesis by (simp add: xs w Lang_of_append Lang_of_Nt)
+      qed
+    qed
+  qed
+  then show "P \<union> Q \<turnstile> xs \<Rightarrow>* map Tm w \<Longrightarrow> P \<union> Expand f Q \<turnstile> xs \<Rightarrow>* map Tm w" for xs w
+    by (auto simp: rtranclp_power Lang_of_iff_derives)
+qed
+
+lemma Lang_Expand_left:
+  assumes f: "\<forall>(A,\<alpha>) \<in> Q. f \<alpha> \<in> Expand_syms_ops P L \<alpha>" and L: "Lhss Q \<subseteq> L"
+  shows "Lang (Expand f Q \<union> P) = Lang (Q \<union> P)"
+  using Lang_Expand[OF f L] by (simp add: ac_simps)
+
+subsubsection \<open>Instance: Expanding all nonterminals\<close>
+
+definition Expand_all_sym :: "('n,'t) Prods \<Rightarrow> 'n set \<Rightarrow> ('n,'t) sym \<Rightarrow> ('n,'t) syms set" where
+"Expand_all_sym P L x = (case x of Nt A \<Rightarrow> if A \<in> L then {[x]} else Rhss P A | _ \<Rightarrow> {[x]})"
+
+lemma Expand_all_sym_ops: "Expand_all_sym P L x \<in> Expand_sym_ops P L x"
+  by (auto simp: Expand_all_sym_def Expand_sym_ops_simps split: sym.splits)
+
+fun Expand_all_syms where
+  "Expand_all_syms P L [] = {[]}"
+| "Expand_all_syms P L (x#xs) = Expand_all_sym P L x @@ Expand_all_syms P L xs"
+
+lemma Expand_all_syms_ops: "Expand_all_syms P L xs \<in> Expand_syms_ops P L xs"
+  by (induction xs, simp, force simp: Expand_all_sym_ops)
+
+abbreviation Expand_all where
+"Expand_all P L Q \<equiv> Expand (Expand_all_syms P L) Q"
+
+lemma Lang_Expand_all:
+  assumes "Lhss Q \<subseteq> L"
+  shows "Lang (Expand_all P L Q \<union> P) = Lang (Q \<union> P)"
+  apply (rule Lang_Expand_left[OF _ assms])
+  by (simp add: Expand_all_syms_ops)
+
+end
